Progress with concurrency lemmas

src/Bisimulations.v
@@ -20,7 +20,7 @@ Proof.
     * eexists. split. 2: reflexivity.
       eapply n_spawn; try eassumption.
     * eexists. split. 2: reflexivity.
-      eapply n_terminate. auto.
+      eapply n_terminate.
   }
   {
     subst. induction H0.
@@ -33,7 +33,7 @@ Proof.
     * eexists. split. 2: reflexivity.
       eapply n_spawn; try eassumption.
     * eexists. split. 2: reflexivity.
-      eapply n_terminate. auto.
+      eapply n_terminate.
   }
 Qed.
 
@@ -133,6 +133,13 @@ Proof.
   * eapply closureNodeSem_trans; eassumption.
 Qed.
 
+Theorem bool_from_lit_val :
+  forall y e, Some y = bool_from_lit e -> VALCLOSED e.
+Proof.
+  destruct e; intros; inversion H.
+  now constructor.
+Qed.
+
 Definition onlyOne (a : Action) (ι : PID) (n n''' : Node) :=
   exists n' n'', n -->* n' /\ n' -[a|ι]ₙ-> n'' /\ n'' -->* n'''.
 
@@ -141,19 +148,25 @@ Lemma internal_determinism :
 Proof.
   intros p p' a IH. induction IH; intros.
   * inversion H0; subst; try (inversion H; inversion_is_value).
-    eapply step_determinism in H. 2: exact H5. destruct H. now subst.
+    - eapply step_determinism in H. 2: exact H7. destruct H. now subst.
   * inversion H1; subst; try inversion_is_value. auto.
+  * inversion H0; now subst.
+  * inversion H0; now subst.
   * inversion H0; now subst.
   * inversion H; now subst.
   * inversion H1; now subst.
-  * inversion H1. subst. rewrite H in H7. now inversion H7.
+  * inversion H1. subst. rewrite H in H9. now inversion H9.
+  * inversion H0; subst.
+    - rewrite <- H in H7. inversion H7. now subst.
+  * inversion H0; subst.
+    - reflexivity.
 Qed.
 
 Lemma par_eq : forall ι p p' Π Π',
   ι : p |||| Π = ι : p' |||| Π' -> p = p'.
 Proof.
   intros. apply equal_f with ι in H as H'.
-  unfold par, update in H'; break_match_hyp. 2: congruence. inversion H'. auto.
+  unfold update in H'; break_match_hyp. 2: congruence. inversion H'. auto.
 Qed.
 
 Lemma concurrent_determinism :
@@ -162,97 +175,117 @@ Proof.
   intros Π a ι Π' IH. inversion IH; intros; subst.
   * inversion H4; subst.
     - apply par_eq in H2 as H2'. subst.
-      eapply internal_determinism in H. 2:exact H7. subst. auto. f_equal.
-      extensionality ι''. apply equal_f with ι'' in H2. unfold par, update in *.
+      eapply internal_determinism in H. 2:exact H8. subst. auto. f_equal.
+      extensionality ι''. apply equal_f with ι'' in H2. unfold update in *.
       break_match_goal; auto.
-    - intuition; try congruence. destruct H3. congruence.
+    - intuition; try congruence. destruct H0. congruence.
   * inversion H5; subst.
     - apply par_eq in H2 as H2'. inversion H2'. subst.
-      eapply internal_determinism in H0. 2: exact H8. subst.
-      f_equal. extensionality ι''. apply equal_f with ι'' in H2. unfold par, update in *.
+      eapply internal_determinism in H0. 2: exact H10. subst.
+      f_equal. extensionality ι''. apply equal_f with ι'' in H2. unfold update in *.
       break_match_goal; auto.
-    - intuition; try congruence. destruct H4. congruence.
+    - intuition; try congruence. destruct H1. congruence.
   * inversion H5; subst.
-    - intuition; try congruence. destruct H0. congruence.
-    - intuition; try congruence. destruct H0. congruence.
+    - intuition; try congruence. destruct H1. congruence.
+    - intuition; try congruence. destruct H1. congruence.
     - apply par_eq in H2 as H2'. subst.
       eapply internal_determinism in H. 2: exact H3. subst. f_equal.
-      extensionality ι''. apply equal_f with ι'' in H2. unfold par, update in *.
+      extensionality ι''. apply equal_f with ι'' in H2. unfold update in *.
       break_match_goal; auto.
-    - intuition; try congruence. destruct H0. congruence.
+    - intuition; try congruence. destruct H1. congruence.
     - apply par_eq in H3 as H3'. subst.
       inversion H; subst; try inversion_is_value.
   * inversion H6; subst.
-    - intuition; try congruence. destruct H5. congruence.
+    - intuition; try congruence. destruct H2. congruence.
     - apply par_eq in H3 as H3'. subst.
       eapply internal_determinism in H1. 2: exact H12. subst.
       f_equal. rewrite H in H10. inversion H10. subst.
-      extensionality ι''. apply equal_f with ι'' in H3. unfold par, update in *.
+      extensionality ι''. apply equal_f with ι'' in H3. unfold update in *.
       break_match_goal; auto.
       break_match_goal; auto.
-  * inversion H4; subst.
-    - apply par_eq in H1 as H1'. subst.
-      inversion H2; subst; try inversion_is_value.
-    - unfold par, update in *. f_equal.
-      extensionality ι'. apply equal_f with ι' in H2. break_match_goal; auto.
+  * inversion H3; subst.
+    - apply par_eq in H0 as H0'. subst.
+      intuition; subst; try congruence. destruct H. congruence.
+      inversion H1.
+    - unfold update in *. f_equal.
+      extensionality ι'. apply equal_f with ι' in H1. break_match_goal; auto.
 Qed.
 
 Lemma internal_equal :
-  forall p p', p -⌈ AInternal ⌉-> p' -> forall p'' a, p -⌈ a ⌉-> p''
+  forall p p', inl p -⌈ AInternal ⌉-> p' -> forall p'' a, inl p -⌈ a ⌉-> p''
 ->
-  (a = AInternal /\ p'' = p') \/ (exists t, a = AArrive t /\ p'' = (p.1.1, p.1.2, p.2 ++ [t])).
+  (a = AInternal /\ p'' = p') \/
+  (exists t ι ι', a = AArrive ι ι' t
+   /\ exists p''', p' -⌈AArrive ι ι' t⌉-> p'''
+  (*  /\ 
+   match p'', t with
+   | inl p'', Message t => p'' = (p.1.1.1.1, p.1.1.1.2, p.1.1.2 ++ [t], p.1.2, p.2)
+   | inl p'', Exit t => 
+   | inl p'', _ => False
+   | inr dp, _  => False
+   end *)).
 Proof.
   intros. inversion H; subst; inversion H0; subst.
-  all: try (inversion H1; subst; inversion_is_value); auto; try inversion_is_value.
-  * eapply step_determinism in H1. 2: exact H7. destruct H1. subst. auto.
-  * right. exists v. auto.
+  all: try (inversion H2; subst; inversion_is_value); auto; try inversion_is_value.
+  * eapply step_determinism in H2. 2: exact H9. destruct H2. subst. auto.
+  * right. exists (Message v),source, dest. auto.
+    split; auto. eexists. constructor; auto.
+  * right. exists (Exit reason),source,dest.
+    split; auto. eexists. constructor; auto.
+  * apply bool_from_lit_val in H9. inversion H2; subst; inversion_is_value.
 Qed.
 
-Definition modifyMailbox (p : PID) (ι0 : PID) (t : Exp) (n : Node) : Node :=
-  let (g, procs) := n in (etherPop (ι0, t) g, 
-                          fun ι => if Nat.eq_dec p ι
-                                   then match procs ι with
-                                         | Some (fs, e, mb) => Some (fs, e, mb ++ [t])
-                                         | None => None
-                                         end
-                                    else procs ι).
+Definition modifyMailbox (p : PID) (ι0 : PID) (ι : PID) (t : Exp) (n : Node) : Node :=
+  let (g, procs) := n in (etherPop (ι0, ι, Message t) g, 
+                      fun ι => if Nat.eq_dec p ι
+                               then match procs ι with
+                                     | Some (inl (fs, e, mb, links, flag)) =>
+                                          Some (inl (fs, e, mb ++ [t], links, flag))
+                                     | r => r
+                                     end
+                                else procs ι).
+
+Theorem internal_is_alive :
+  forall p p', p -⌈AInternal⌉-> p' -> exists pa, p = inl pa.
+Proof.
+  intros. inversion H; subst; try (do 2 eexists; split; reflexivity).
+Qed.
 
 Lemma internal_det :
   forall n n' n'' ι a, n -[AInternal | ι]ₙ-> n' -> n -[a | ι]ₙ-> n''
 ->
-  (a = AInternal /\ n''= n') \/ (exists t, a = AArrive t /\
+  (a = AInternal /\ n''= n') \/ (exists t ι', a = AArrive ι' ι t /\
+                                 exists n''', n' -[AArrive ι' ι t | ι]ₙ-> n'''
+  
+                                (* /\
                                  n'' = modifyMailbox ι ι t n /\
                                  exists n''', n' -[AArrive t | ι]ₙ-> n''' /\
-                                 n''' = modifyMailbox ι ι t n').
+                                 n''' = modifyMailbox ι ι t n' *)).
 Proof.
   intros. inversion H; inversion H0; subst.
   * inversion H8; subst. apply par_eq in H5. subst.
-    eapply internal_equal in H7; eauto. destruct H7 as [[? ?] | [? [? ?]]]; congruence.
-  * right. inversion H9; subst. apply par_eq in H5; subst.
-    eapply internal_equal in H8 as H8'. 2: exact H1.
-    destruct H8' as [[? ?] | [? [? ?]]]; try congruence.
-    destruct p,p. simpl in H4. subst. exists t.
-    split; auto. split.
-    - simpl. f_equal.
-      unfold par, update. inversion H3. subst.
-      extensionality ι'.
-      break_match_goal; auto.
-    - simpl. inversion H3. subst.
-      exists (etherPop (ι, x) ether, ι : (p'.1.1, p'.1.2, p'.2 ++ [x]) |||| Π).
-      split.
-      + apply n_arrive; auto. destruct p', p. simpl. apply p_arrive; auto.
-        inversion H8; auto.
-      + f_equal. extensionality ι'. unfold par, update. break_match_goal; simpl.
-        destruct p',p. auto. auto.
+    apply internal_is_alive in H1 as H1'. destruct H1'. subst.
+    eapply internal_equal in H7; eauto.
+    destruct H7 as [[? ?] | [? [? [? [? ?]]]]];  congruence.
   * inversion H9; subst. apply par_eq in H5; subst.
-    eapply internal_equal in H7. 2: exact H1. destruct H7 as [[? ?] | [? [? ?]]]; try congruence.
+    eapply internal_is_alive in H1 as H1'. destruct H1'. subst.
+    eapply internal_equal in H8 as H8'. 2: exact H1.
+    destruct H8' as [[? ?] | [? [? [? [? [? ?]]]]]]; try congruence.
+    inversion H3. subst. right.
+    do 2 eexists. split. reflexivity.
+    eexists. econstructor; eauto.
+  * inversion H9; subst. apply par_eq in H5; subst.
+    apply internal_is_alive in H1 as H1'. destruct H1'. subst.
+    eapply internal_equal in H7. 2: exact H1. destruct H7 as [[? ?] | [? [? [? [? [? ?]]]]]]; try congruence.
     - subst. left; split; auto. f_equal. inversion H9.
-      extensionality x. apply equal_f with x in H4. unfold par, update in *. break_match_goal; auto.
-    - subst. inversion H8. 2: inversion H3. 3: destruct H4. all: try congruence.
+      extensionality x'. apply equal_f with x' in H4. unfold update in *. break_match_goal; auto.
+    - subst. inversion H8. 2: destruct H3. 3: destruct H3.
+      3-4: destruct H3. all: try congruence.
   * inversion H10; subst. apply par_eq in H5. subst.
-    eapply internal_equal in H9; eauto. destruct H9 as [[? ?] | [? [? ?]]]; congruence.
-  * inversion H8; subst. apply par_eq in H5. subst.
-    inversion H1; subst; try inversion_is_value. now apply value_nostep in H9.
+    apply internal_is_alive in H1 as H1'. destruct H1'. subst.
+    eapply internal_equal in H9; eauto. destruct H9 as [[? ?] | [? [? [? [? ?]]]]]; congruence.
+  * inversion H7; subst. apply par_eq in H5. subst.
+    inversion H1; subst; try inversion_is_value.
 Qed.
 
 Definition bothSpawn (a1 a2 : Action) : Prop:=
@@ -270,118 +303,120 @@ Lemma step_chain :
 Proof.
   intros n n' ι a IH. inversion IH; intros; subst.
   * inversion H4; subst.
-    - exists ((ether ++ [(ι', t)]) ++ [(ι'1, t0)], ι'0 : p'0 |||| ι : p' |||| prs ).
+    - exists ((ether ++ [(ι, ι', t)]) ++ [(ι'0, ι'1, t0)], ι'0 : p'0 |||| ι : p' |||| prs ).
       replace (ι : p' |||| prs) with (ι'0 : p0 |||| ι : p' |||| prs) at 1.
-      2: { extensionality ι1. unfold par, update in *. apply equal_f with ι1 in H2.
+      2: { extensionality ι1. unfold update in *. apply equal_f with ι1 in H2.
            break_match_goal; subst.
            break_match_goal; subst. congruence. auto.
            auto.
          }
       now constructor.
-    - exists (etherPop (ι'0, t0) (ether ++ [(ι', t)])
+    - exists (etherPop (ι1, ι'0, t0) (ether ++ [(ι, ι', t)])
               , ι'0 : p'0 |||| ι : p' |||| prs ).
       replace (ι : p' |||| prs) with (ι'0 : p0 |||| ι : p' |||| prs) at 1.
-      2: { extensionality ι1. unfold par, update in *. apply equal_f with ι1 in H1.
+      2: { extensionality x. unfold update in *. apply equal_f with x in H1.
            break_match_goal; subst.
            break_match_goal; subst. congruence. auto.
            auto.
          }
       constructor. 2: auto.
       apply in_or_app. now left.
-    - exists (ether ++ [(ι', t)], ι'0 : p'0 |||| ι : p' |||| prs).
+    - exists (ether ++ [(ι, ι', t)], ι'0 : p'0 |||| ι : p' |||| prs).
       replace (ι : p' |||| prs) with (ι'0 : p0 |||| ι : p' |||| prs) at 1.
-      2: { extensionality ι1. unfold par, update in *. apply equal_f with ι1 in H1.
+      2: { extensionality x. unfold update in *. apply equal_f with x in H1.
            break_match_goal; subst.
            break_match_goal; subst. congruence. auto.
            auto.
          }
       now constructor.
-    - exists (ether ++ [(ι', t)], 
-              ι'1 : ([], EApp v1 l, []) |||| ι'0 : p'0 |||| ι : p' |||| prs).
+    - exists (ether ++ [(ι, ι', t)], 
+              ι'1 : inl ([], EApp v1 l, [], [], false) |||| ι'0 : p'0 |||| ι : p' |||| prs).
       replace (ι : p' |||| prs) with (ι'0 : p0 |||| ι : p' |||| prs) at 1.
-      2: { extensionality ι1. unfold par, update in *. apply equal_f with ι1 in H1.
+      2: { extensionality x. unfold update in *. apply equal_f with x in H1.
            break_match_goal; subst.
            break_match_goal; subst. congruence. auto.
            auto.
          }
       constructor; auto.
       apply equal_f with ι'1 in H1.
-      unfold par, update in *. break_match_goal; auto.
+      unfold update in *. break_match_goal; auto.
       break_match_goal; subst.
       + congruence.
       + now rewrite H1 in H3.
-    - exists (ether ++ [(ι', t)],
+    - exists (ether ++ [(ι, ι', t)],
                ι : p' |||| prs -- ι'0).
-      replace (ι : p' |||| prs) with (ι'0 : ([], v, mb) |||| ι : p' |||| prs) at 1.
-      2: { extensionality ι1. unfold par, update in *. apply equal_f with ι1 in H2.
+      replace (ι : p' |||| prs) with (ι'0 : inr [] |||| ι : p' |||| prs) at 1.
+      2: { extensionality x. unfold update in *. apply equal_f with x in H2.
            break_match_goal; subst.
            break_match_goal; subst. congruence. auto.
            auto.
          }
+      rewrite update_swap with (ι := ι); auto.
       constructor; auto.
   * inversion H5; subst.
-    - exists (etherPop (ι, t) ether ++ [(ι'0, t0)], ι' : p'0 |||| ι : p' |||| prs).
+    - exists (etherPop (ι1, ι, t) ether ++ [(ι', ι'0, t0)], ι' : p'0 |||| ι : p' |||| prs).
       replace (ι : p' |||| prs) with (ι' : p0 |||| ι : p' |||| prs) at 1.
-      2: { extensionality ι1. unfold par, update in *. apply equal_f with ι1 in H3.
+      2: { extensionality x. unfold update in *. apply equal_f with x in H3.
            break_match_goal; subst.
            break_match_goal; subst. congruence. auto.
            auto.
          }
       now constructor.
-    - exists (etherPop (ι', t0) (etherPop (ι, t) ether)
+    - exists (etherPop (ι2, ι', t0) (etherPop (ι1, ι, t) ether)
               , ι' : p'0 |||| ι : p' |||| prs ).
       replace (ι : p' |||| prs) with (ι' : p0 |||| ι : p' |||| prs) at 1.
-      2: { extensionality ι1. unfold par, update in *. apply equal_f with ι1 in H2.
+      2: { extensionality x. unfold update in *. apply equal_f with x in H2.
            break_match_goal; subst.
            break_match_goal; subst. congruence. auto.
            auto.
          }
       constructor. 2: auto.
       apply removeFirst_In; auto. intro. apply H6. now inversion H1.
-    - exists ((etherPop (ι, t) ether), ι' : p'0 |||| ι : p' |||| prs).
+    - exists ((etherPop (ι1, ι, t) ether), ι' : p'0 |||| ι : p' |||| prs).
       replace (ι : p' |||| prs) with (ι' : p0 |||| ι : p' |||| prs) at 1.
-      2: { extensionality ι1. unfold par, update in *. apply equal_f with ι1 in H2.
+      2: { extensionality x. unfold update in *. apply equal_f with x in H2.
            break_match_goal; subst.
            break_match_goal; subst. congruence. auto.
            auto.
          }
       now constructor.
-    - exists ((etherPop (ι, t) ether), 
-              ι'0 : ([], EApp v1 l, []) |||| ι' : p'0 |||| ι : p' |||| prs).
+    - exists ((etherPop (ι1, ι, t) ether), 
+              ι'0 : inl ([], EApp v1 l, [], [], false) |||| ι' : p'0 |||| ι : p' |||| prs).
       replace (ι : p' |||| prs) with (ι' : p0 |||| ι : p' |||| prs) at 1.
-      2: { extensionality ι1. unfold par, update in *. apply equal_f with ι1 in H2.
+      2: { extensionality x. unfold update in *. apply equal_f with x in H2.
            break_match_goal; subst.
            break_match_goal; subst. congruence. auto.
            auto.
          }
       constructor; auto.
       apply equal_f with ι'0 in H2.
-      unfold par, update in *. break_match_goal; auto.
+      unfold update in *. break_match_goal; auto.
       break_match_goal; subst.
       + congruence.
       + now rewrite H2 in H4.
-    - exists (etherPop (ι, t) ether,
+    - exists (etherPop (ι1, ι, t) ether,
                ι : p' |||| prs -- ι').
-      replace (ι : p' |||| prs) with (ι' : ([], v, mb) |||| ι : p' |||| prs) at 1.
-      2: { extensionality ι1. unfold par, update in *. apply equal_f with ι1 in H3.
+      replace (ι : p' |||| prs) with (ι' : inr [] |||| ι : p' |||| prs) at 1.
+      2: { extensionality x. unfold update in *. apply equal_f with x in H3.
            break_match_goal; subst.
            break_match_goal; subst. congruence. auto.
            auto.
          }
+      rewrite update_swap with (ι := ι); auto.
       constructor; auto.
   * inversion H5; subst.
-    - exists (ether ++ [(ι'0, t)], ι' : p'0 |||| ι : p' |||| Π).
+    - exists (ether ++ [(ι', ι'0, t)], ι' : p'0 |||| ι : p' |||| Π).
       replace (ι : p' |||| Π) with (ι' : p0 |||| ι : p' |||| Π) at 1.
-      2: { extensionality ι1. unfold par, update in *. apply equal_f with ι1 in H3.
+      2: { extensionality x. unfold update in *. apply equal_f with x in H3.
            break_match_goal; subst.
            break_match_goal; subst. congruence. auto.
            auto.
          }
       now constructor.
-    - exists (etherPop (ι', t) ether
+    - exists (etherPop (ι1, ι', t) ether
               , ι' : p'0 |||| ι : p' |||| Π ).
       replace (ι : p' |||| Π) with (ι' : p0 |||| ι : p' |||| Π) at 1.
-      2: { extensionality ι1. unfold par, update in *. apply equal_f with ι1 in H2.
+      2: { extensionality x. unfold update in *. apply equal_f with x in H2.
            break_match_goal; subst.
            break_match_goal; subst. congruence. auto.
            auto.
@@ -389,59 +424,64 @@ Proof.
       constructor; auto.
     - exists (ether, ι' : p'0 |||| ι : p' |||| Π).
       replace (ι : p' |||| Π) with (ι' : p0 |||| ι : p' |||| Π) at 1.
-      2: { extensionality ι1. unfold par, update in *. apply equal_f with ι1 in H2.
+      2: { extensionality x. unfold update in *. apply equal_f with x in H2.
            break_match_goal; subst.
            break_match_goal; subst. congruence. auto.
            auto.
          }
       now constructor.
     - exists (ether, 
-              ι'0 : ([], EApp v1 l, []) |||| ι' : p'0 |||| ι : p' |||| Π).
+              ι'0 : inl ([], EApp v1 l, [], [], false) |||| ι' : p'0 |||| ι : p' |||| Π).
       replace (ι : p' |||| Π) with (ι' : p0 |||| ι : p' |||| Π) at 1.
-      2: { extensionality ι1. unfold par, update in *. apply equal_f with ι1 in H2.
+      2: { extensionality x. unfold update in *. apply equal_f with x in H2.
            break_match_goal; subst.
            break_match_goal; subst. congruence. auto.
            auto.
          }
       constructor; auto.
       apply equal_f with ι'0 in H2.
-      unfold par, update in *. break_match_goal; auto.
+      unfold update in *. break_match_goal; auto.
       break_match_goal; subst.
       + congruence.
       + now rewrite H2 in H4.
     - exists (ether,
                ι : p' |||| Π -- ι').
-      replace (ι : p' |||| Π) with (ι' : ([], v, mb) |||| ι : p' |||| Π) at 1.
-      2: { extensionality ι1. unfold par, update in *. apply equal_f with ι1 in H3.
+      replace (ι : p' |||| Π) with (ι' : inr [] |||| ι : p' |||| Π) at 1.
+      2: { extensionality ι1. unfold update in *. apply equal_f with ι1 in H3.
            break_match_goal; subst.
            break_match_goal; subst. congruence. auto.
            auto.
          }
+      rewrite update_swap with (ι := ι); auto.
       constructor; auto.
   * inversion H6; subst.
-    - exists (ether ++ [(ι'1, t)], ι'0 : p'0 |||| ι' : ([], EApp v1 l, []) |||| ι : p' |||| Π).
-      replace (ι' : ([], EApp v1 l, []) |||| ι : p' |||| Π) with 
-              (ι'0 : p0 |||| ι' : ([], EApp v1 l, []) |||| ι : p' |||| Π) at 1.
-      2: { extensionality ι1. unfold par, update in *. apply equal_f with ι1 in H4.
+    - exists (ether ++ [(ι'0, ι'1, t)], ι'0 : p'0 |||| 
+                                        ι' : inl ([], EApp v1 l, [], [], false) |||| 
+                                        ι : p' |||| Π).
+      replace (ι' : inl ([], EApp v1 l, [], [], false) |||| ι : p' |||| Π) with 
+              (ι'0 : p0 |||| ι' : inl ([], EApp v1 l, [], [], false) |||| ι : p' |||| Π) at 1.
+      2: { extensionality x. unfold update in *. apply equal_f with x in H4.
            break_match_goal; subst;
            break_match_goal; subst; auto.
            all: break_match_hyp; auto; congruence.
          }
       now constructor.
-    - exists (etherPop (ι'0, t) ether
-              , ι'0 : p'0 |||| ι' : ([], EApp v1 l, []) |||| ι : p' |||| Π ).
-      replace (ι' : ([], EApp v1 l, []) |||| ι : p' |||| Π) with 
-              (ι'0 : p0 |||| ι' : ([], EApp v1 l, []) |||| ι : p' |||| Π) at 1.
-      2: { extensionality ι1. unfold par, update in *. apply equal_f with ι1 in H3.
+    - exists (etherPop (ι1, ι'0, t) ether
+              , ι'0 : p'0 |||| ι' : inl ([], EApp v1 l, [], [], false) 
+                          |||| ι : p' |||| Π ).
+      replace (ι' : inl ([], EApp v1 l, [], [], false) |||| ι : p' |||| Π) with 
+              (ι'0 : p0 |||| ι' : inl ([], EApp v1 l, [], [], false) |||| ι : p' |||| Π) at 1.
+      2: { extensionality x. unfold update in *. apply equal_f with x in H3.
            break_match_goal; subst;
            break_match_goal; subst; auto.
            all: break_match_hyp; auto; try congruence.
          }
       constructor; auto.
-    - exists (ether, ι'0 : p'0 |||| ι' : ([], EApp v1 l, []) |||| ι : p' |||| Π).
-      replace (ι' : ([], EApp v1 l, []) |||| ι : p' |||| Π) with 
-              (ι'0 : p0 |||| ι' : ([], EApp v1 l, []) |||| ι : p' |||| Π) at 1.
-      2: { extensionality ι1. unfold par, update in *. apply equal_f with ι1 in H3.
+    - exists (ether, ι'0 : p'0 |||| ι' : inl ([], EApp v1 l, [], [], false)
+                               |||| ι : p' |||| Π).
+      replace (ι' : inl ([], EApp v1 l, [], [], false) |||| ι : p' |||| Π) with 
+              (ι'0 : p0 |||| ι' : inl ([], EApp v1 l, [], [], false) |||| ι : p' |||| Π) at 1.
+      2: { extensionality x. unfold update in *. apply equal_f with x in H3.
            break_match_goal; subst;
            break_match_goal; subst; auto.
            all: break_match_hyp; auto; congruence.
@@ -450,29 +490,35 @@ Proof.
     - (** cannot be sure to generate different spawn PID-s *)
       exfalso. apply Spawns. cbn. auto.
     - exists (ether,
-               ι' : ([], EApp v1 l, []) |||| ι : p' |||| Π -- ι'0).
-      replace (ι' : ([], EApp v1 l, []) |||| ι : p' |||| Π) with 
-              (ι'0 : ([], v, mb) |||| ι' : ([], EApp v1 l, []) |||| ι : p' |||| Π) at 1.
-      2: { extensionality ι1. unfold par, update in *. apply equal_f with ι1 in H4.
+               ι' : inl ([], EApp v1 l, [], [], false) |||| ι : p' |||| Π -- ι'0).
+      replace (ι' : inl ([], EApp v1 l, [], [], false) |||| ι : p' |||| Π) with 
+              (ι'0 : inr [] |||| ι' : inl ([], EApp v1 l, [], [], false) 
+                            |||| ι : p' |||| Π) at 1.
+      2: { extensionality x. unfold update in *. apply equal_f with x in H4.
            break_match_goal; subst.
            break_match_goal; subst. congruence.
            break_match_goal; auto. congruence.
            break_match_goal; auto.
          }
+      rewrite update_swap with (ι := ι); auto.
+      rewrite update_swap with (ι := ι') (ι' := ι'0); auto.
       constructor; auto.
-  * inversion H4; subst.
-    - exists (ether ++ [(ι'0, t)], ι' : p' |||| (Π -- ι)).
+      apply equal_f with ι' in H4. unfold update in H4. cbn in H4.
+      break_match_hyp; auto; subst. break_match_hyp; subst; try congruence; auto.
+      unfold update in H0. break_match_hyp; congruence.
+  * inversion H3; subst.
+    - exists (ether ++ [(ι', ι'0, t)], ι' : p' |||| (Π -- ι)).
       replace (Π -- ι) with (ι' : p |||| (Π -- ι)) at 1.
-      2: { extensionality ι1. unfold par, update in *. apply equal_f with ι1 in H2.
+      2: { extensionality x. unfold update in *. apply equal_f with x in H1.
            break_match_goal; subst.
            break_match_goal; subst. congruence. auto.
            auto.
          }
       now constructor.
-    - exists (etherPop (ι', t) ether
+    - exists (etherPop (ι1, ι', t) ether
               , ι' : p' |||| (Π -- ι) ).
       replace (Π -- ι) with (ι' : p |||| (Π -- ι)) at 1.
-      2: { extensionality ι1. unfold par, update in *. apply equal_f with ι1 in H1.
+      2: { extensionality x. unfold update in *. apply equal_f with x in H0.
            break_match_goal; subst.
            break_match_goal; subst. congruence. auto.
            auto.
@@ -480,27 +526,27 @@ Proof.
       constructor; auto.
     - exists (ether, ι' : p' |||| (Π -- ι)).
       replace (Π -- ι) with (ι' : p |||| (Π -- ι)) at 1.
-      2: { extensionality ι1. unfold par, update in *. apply equal_f with ι1 in H1.
+      2: { extensionality x. unfold update in *. apply equal_f with x in H0.
            break_match_goal; subst.
            break_match_goal; subst. congruence. auto.
            auto.
          }
       now constructor.
     - exists (ether, 
-              ι'0 : ([], EApp v1 l, []) |||| ι' : p' |||| (Π -- ι)).
+              ι'0 : inl ([], EApp v1 l, [], [], false) |||| ι' : p' |||| (Π -- ι)).
       replace (Π -- ι) with (ι' : p |||| (Π -- ι)) at 1.
-      2: { extensionality ι1. unfold par, update in *. apply equal_f with ι1 in H1.
+      2: { extensionality x. unfold update in *. apply equal_f with x in H0.
            break_match_goal; subst.
            break_match_goal; subst. congruence. auto.
            auto.
          }
       constructor; auto.
-      apply equal_f with ι'0 in H1.
-      unfold par, update in *. break_match_goal; auto.
+      apply equal_f with ι'0 in H0.
+      unfold update in *. break_match_goal; auto.
       break_match_goal; subst; auto. congruence.
     - exists (ether, (Π -- ι) -- ι').
-      replace (Π -- ι) with (ι' : ([], v0, mb0) |||| (Π -- ι)) at 1.
-      2: { extensionality ι1. unfold par, update in *. apply equal_f with ι1 in H2.
+      replace (Π -- ι) with (ι' : inr [] |||| (Π -- ι)) at 1.
+      2: { extensionality x. unfold update in *. apply equal_f with x in H1.
            break_match_goal; subst. auto.
            break_match_goal; subst. congruence. auto.
            break_match_goal; subst; auto.
@@ -529,12 +575,20 @@ Proof.
         split. 2: split. constructor.
         auto.
         split; auto.
-      + destruct H0' as [eq1 [eq2 [newn [D eq3]]]]. subst.
-        eapply IHSteps in H5 as H5'. 2: exact D.
-        destruct H5' as [[n3 [n4 [l1 [l2 [k1 [k2 H2]]]]]]| [n3 D2]].
-        ** left. destruct H2 as [eq1 [D1 [D2 [ D3 [eq2 eq3]]]]]. subst.
-           congruence.
-        ** right. eexists; eauto.
+      + destruct H0' as [source [eq [n''' D]]]. subst.
+        inversion H1; subst.
+        2: { intuition; try congruence. destruct H4; congruence. }
+        inversion H10; subst.
+        ** specialize (IHSteps H5 _ _ _ D).
+           destruct IHSteps as [[n3 [n4 [l1 [l2 [k1 [k2 H2]]]]]]| [n3 D2]].
+           -- left. destruct H2 as [eq1 [D1 [D2 [ D3 [eq2 eq3]]]]]. subst.
+              congruence.
+           -- right. eexists; eauto.
+        ** specialize (IHSteps H5 _ _ _ D).
+           destruct IHSteps as [[n3 [n4 [l1 [l2 [k1 [k2 H2]]]]]]| [n3 D2]].
+           -- left. destruct H2 as [eq1 [D1 [D2 [ D3 [eq2 eq3]]]]]. subst.
+              congruence.
+           -- right. eexists; eauto.
     - eapply step_chain in H1. 2: exact H. 2-3: auto.
       destruct H1. eapply IHSteps in H1 as H1'; auto.
       destruct H1' as [[n3 [n4 [l1 [l2 [k1 H2]]]]] | [t H0']]; subst.
@@ -551,7 +605,7 @@ Lemma internal_keep :
   forall x, x <> ι -> snd n x = snd n' x.
 Proof.
   intros. inversion H; subst.
-  simpl. unfold par, update. break_match_goal; auto. congruence.
+  simpl. unfold update. break_match_goal; auto. congruence.
 Qed.
 
 (* general case wont work: message ordering is desructed *)
@@ -565,114 +619,134 @@ Proof.
   inversion H2; subst.
   * inversion H1; subst.
     inversion H0; subst.
-    2: { intuition; try congruence. destruct H5; congruence. }
-    assert (p = p0). {
-      apply internal_keep with (x := ι2) in H0. simpl in H0.
-      unfold par, update in H0. break_match_hyp. now inversion H0. congruence.
-      auto.
-    }
-    subst.
-    subst. eapply internal_determinism in H3. 2: exact H9. subst.
-    assert ((ι1 : p1 |||| ι2 : p' |||| prs0) = ι1 : p1 |||| ι2 : p' |||| prs) as EQ. {
-      extensionality x. unfold par, update in *. break_match_goal; auto.
-      apply internal_keep with (x := x) in H0. simpl in H0.
-      break_match_goal; auto. auto.
-    }
-    replace (ι2 : p' |||| prs0) with (ι1 : p1 |||| ι2 : p' |||| prs0).
-    replace (ι2 : p' |||| prs) with (ι1 : p'1 |||| ι2 : p' |||| prs).
-    rewrite EQ. constructor; auto.
-    all: unfold par, update in *; extensionality x; 
-         apply equal_f with x in H5; apply equal_f with x in H11;
-         do 2 break_match_goal; subst; auto; congruence.
-  * inversion H1; subst.
-    inversion H0; subst.
     2: { intuition; try congruence. destruct H6; congruence. }
     assert (p = p0). {
       apply internal_keep with (x := ι2) in H0. simpl in H0.
-      unfold par, update in H0. break_match_hyp. now inversion H0. congruence.
+      unfold update in H0. break_match_hyp. now inversion H0. congruence.
       auto.
     }
     subst.
-    subst. eapply internal_determinism in H4. 2: exact H8. subst.
+    subst. eapply internal_determinism in H3. 2: exact H10. subst.
     assert ((ι1 : p1 |||| ι2 : p' |||| prs0) = ι1 : p1 |||| ι2 : p' |||| prs) as EQ. {
-      extensionality x. unfold par, update in *. break_match_goal; auto.
+      extensionality x. unfold update in *. break_match_goal; auto.
       apply internal_keep with (x := x) in H0. simpl in H0.
       break_match_goal; auto. auto.
     }
     replace (ι2 : p' |||| prs0) with (ι1 : p1 |||| ι2 : p' |||| prs0).
     replace (ι2 : p' |||| prs) with (ι1 : p'1 |||| ι2 : p' |||| prs).
     rewrite EQ. constructor; auto.
-    all: unfold par, update in *; extensionality x; 
-         apply equal_f with x in H7; apply equal_f with x in H13;
+    all: unfold update in *; extensionality x; 
+         apply equal_f with x in H5; apply equal_f with x in H12;
          do 2 break_match_goal; subst; auto; congruence.
   * inversion H1; subst.
-    1,2,4,5: intuition; try congruence; destruct H4; congruence.
     inversion H0; subst.
+    2: { intuition; try congruence. destruct H7; congruence. }
     assert (p = p0). {
       apply internal_keep with (x := ι2) in H0. simpl in H0.
-      unfold par, update in H0. break_match_hyp. now inversion H0. congruence.
+      unfold update in H0. break_match_hyp. now inversion H0. congruence.
       auto.
     }
     subst.
-    subst. eapply internal_determinism in H3. 2: exact H5. subst.
-    assert ((ι1 : p1 |||| ι2 : p' |||| Π0) = ι1 : p1 |||| ι2 : p' |||| Π) as EQ. {
-      extensionality x. unfold par, update in *. break_match_goal; auto.
+    subst. eapply internal_determinism in H4. 2: exact H12. subst.
+    assert ((ι1 : p1 |||| ι2 : p' |||| prs0) = ι1 : p1 |||| ι2 : p' |||| prs) as EQ. {
+      extensionality x. unfold update in *. break_match_goal; auto.
       apply internal_keep with (x := x) in H0. simpl in H0.
       break_match_goal; auto. auto.
     }
-    replace (ι2 : p' |||| Π0) with (ι1 : p1 |||| ι2 : p' |||| Π0).
-    replace (ι2 : p' |||| Π) with (ι1 : p'1 |||| ι2 : p' |||| Π).
+    replace (ι2 : p' |||| prs0) with (ι1 : p1 |||| ι2 : p' |||| prs0).
+    replace (ι2 : p' |||| prs) with (ι1 : p'1 |||| ι2 : p' |||| prs).
     rewrite EQ. constructor; auto.
-    1-2: unfold par, update in *; extensionality x; 
-         apply equal_f with x in H8; apply equal_f with x in H13;
+    all: unfold update in *; extensionality x; 
+         apply equal_f with x in H6; apply equal_f with x in H14;
          do 2 break_match_goal; subst; auto; congruence.
   * inversion H1; subst.
-    1: intuition; try congruence; destruct H7; congruence.
+    1,2,4,5: intuition; try congruence;
+      match goal with
+      | [H : exists _, _ |- _] => destruct H; congruence
+      | _ => idtac
+      end.
+    - inversion H0; subst.
+      assert (p = inr []). {
+        apply internal_keep with (x := ι2) in H0. simpl in H0.
+        unfold update in H0. break_match_hyp. now inversion H0. congruence.
+        auto.
+      }
+      subst.
+      inversion H3.
+    - inversion H0; subst.
+      assert (p = p0). {
+        apply internal_keep with (x := ι2) in H0. simpl in H0.
+        unfold update in H0. break_match_hyp. now inversion H0. congruence.
+        auto.
+      }
+      subst.
+      subst. eapply internal_determinism in H3. 2: exact H5. subst.
+      assert ((ι1 : p1 |||| ι2 : p' |||| Π0) = ι1 : p1 |||| ι2 : p' |||| Π) as EQ. {
+        extensionality x. unfold update in *. break_match_goal; auto.
+        apply internal_keep with (x := x) in H0. simpl in H0.
+        break_match_goal; auto. auto.
+      }
+      replace (ι2 : p' |||| Π0) with (ι1 : p1 |||| ι2 : p' |||| Π0).
+      replace (ι2 : p' |||| Π) with (ι1 : p'1 |||| ι2 : p' |||| Π).
+      rewrite EQ. constructor; auto.
+      1-2: unfold update in *; extensionality x; 
+           apply equal_f with x in H8; apply equal_f with x in H13;
+           do 2 break_match_goal; subst; auto; congruence.
+  * inversion H1; subst.
+    1: intuition; try congruence; destruct H8; congruence.
     inversion H0; subst.
     assert (p = p0). {
       apply internal_keep with (x := ι2) in H0. simpl in H0.
-      unfold par, update in H0. break_match_hyp. now inversion H0. congruence.
+      unfold update in H0. break_match_hyp. now inversion H0. congruence.
       auto.
     }
     subst.
     subst. eapply internal_determinism in H5. 2: exact H14. subst.
-    assert ((ι1 : p1 |||| ι' : ([], EApp v1 l0, []) |||| ι2 : p' |||| Π0) = 
-             ι1 : p1 |||| ι' : ([], EApp v1 l0, []) |||| ι2 : p' |||| Π) as EQ. {
-      extensionality x. unfold par, update in *. break_match_goal; auto.
+    assert ((ι1 : p1 |||| ι' : inl ([], EApp v1 l0, [], [], false) |||| ι2 : p' |||| Π0) = 
+             ι1 : p1 |||| ι' : inl ([], EApp v1 l0, [], [], false) |||| ι2 : p' |||| Π) as EQ. {
+      extensionality x. unfold update in *. break_match_goal; auto.
       break_match_goal; auto.
       apply internal_keep with (x := x) in H0. simpl in H0.
       break_match_goal; auto.
       auto.
     }
     rewrite H3 in H10. inversion H10. subst.
-    replace (ι' : ([], EApp v1 l0, []) |||| ι2 : p' |||| Π0) with
-            (ι1 : p1 |||| ι' : ([], EApp v1 l0, []) |||| ι2 : p' |||| Π0).
-    replace (ι' : ([], EApp v1 l0, []) |||| ι2 : p' |||| Π) with
-            (ι1 : p'1 |||| ι' : ([], EApp v1 l0, []) |||| ι2 : p' |||| Π).
+    replace (ι' : inl ([], EApp v1 l0, [], [], false) |||| ι2 : p' |||| Π0) with
+            (ι1 : p1 |||| ι' : inl ([], EApp v1 l0, [], [], false) |||| ι2 : p' |||| Π0).
+    replace (ι' : inl ([], EApp v1 l0, [], [], false) |||| ι2 : p' |||| Π) with
+            (ι1 : p'1 |||| ι' : inl ([], EApp v1 l0, [], [], false) |||| ι2 : p' |||| Π).
     rewrite EQ. apply n_other; auto.
     clear EQ H1 H2 H0.
-    all: unfold par, update in *; extensionality x;
+    all: unfold update in *; extensionality x;
          apply equal_f with x in H7; apply equal_f with x in H15;
          do 2 break_match_goal; subst; auto; try congruence.
     - break_match_goal; auto. subst. congruence.
     - break_match_goal; auto. subst. congruence.
   * inversion H1; subst.
-    1: intuition; try congruence; destruct H5; congruence.
-    inversion H0. subst.
-    assert ((ι1 : p |||| (Π0 -- ι2)) = 
-             ι1 : p |||| (Π  -- ι2)) as EQ. {
-      extensionality x. unfold par, update in *. break_match_goal; auto.
-      apply internal_keep with (x := x) in H0. simpl in H0.
-      break_match_goal; auto. auto.
-    }
-    replace (Π0 -- ι2) with
-            (ι1 : p |||| (Π0 -- ι2)).
-    replace (Π -- ι2) with
-            (ι1 : p' |||| (Π -- ι2)).
-    rewrite EQ. constructor; auto.
-    all: unfold par, update in *; extensionality x;
-     apply equal_f with x in H6; apply equal_f with x in H11;
-     do 2 break_match_goal; subst; auto; try congruence.
+    1: intuition; try congruence. destruct H5; congruence.
+    - inversion H0; subst.
+      assert (p = inr []). {
+        apply internal_keep with (x := ι2) in H0. simpl in H0.
+        unfold update in H0. break_match_hyp. now inversion H0. congruence.
+        auto.
+      }
+      subst.
+      inversion H3.
+    - inversion H0. subst.
+      assert ((ι1 : p |||| (Π0 -- ι2)) = 
+               ι1 : p |||| (Π  -- ι2)) as EQ. {
+        extensionality x. unfold update in *. break_match_goal; auto.
+        apply internal_keep with (x := x) in H0. simpl in H0.
+        break_match_goal; auto. auto.
+      }
+      replace (Π0 -- ι2) with
+              (ι1 : p |||| (Π0 -- ι2)).
+      replace (Π -- ι2) with
+              (ι1 : p' |||| (Π -- ι2)).
+      rewrite EQ. constructor; auto.
+      all: unfold update in *; extensionality x;
+       apply equal_f with x in H4; apply equal_f with x in H9;
+       do 2 break_match_goal; subst; auto; try congruence.
 Qed.
 
 Theorem delay_internal_same :
@@ -684,28 +758,17 @@ Theorem delay_internal_same :
 Proof.
   intros. inversion H; subst.
   eapply internal_det in H1 as H1'. 2: exact H.
-  destruct H1' as [[eq1 eq2]| [t [eq1 [eq2 [n4 [D eq3]]]]]]; subst.
+  destruct H1' as [[eq1 eq2]| [t [? [eq [n'' D]]]]]; subst.
   * auto.
   * inversion H0; subst.
-    2: { intuition; try congruence; destruct H7; congruence. }
+    2: { intuition; try congruence; destruct H3; congruence. }
     simpl. apply par_eq in H5 as H5'. subst.
-    replace (fun ι0 : nat =>
-              if Nat.eq_dec ι ι0
-              then
-               match (ι : p |||| Π) ι0 with
-               | Some (fs, e, mb) => Some (fs, e, mb ++ [t])
-               | None => None
-               end
-              else (ι : p |||| Π) ι0) with
-             (ι : (fst (fst p), snd (fst p), snd p ++ [t]) |||| prs).
-    2: { extensionality x. unfold par, update in *. apply equal_f with x in H5.
-         break_match_goal; auto.
-         destruct p, p; subst. inversion H10; subst; auto.
-       }
-    apply n_other. 2: now left.
-    inversion H10; subst.
-    inversion H2; simpl; subst.
-    - constructor; auto.
+    inversion H1; subst.
+    - simpl. apply par_eq in H6 as H5'. subst.
+      apply n_other. 2: now left.
+      inversion H10; subst.
+      inversion H2; simpl; subst.
+      - constructor; auto.
 Qed.
 
 Corollary chain_to_front_iff :
@@ -797,13 +860,13 @@ Proof.
 Qed.
 
 Goal Node_equivalence ([], 
-                         0 : ([], ELet "X"%string (ELit 0%Z) (EVar 0), []) ||||
-                         1 : ([], EConcBIF (ELit "send"%string) [EPid 0;ELit 1%Z], []) ||||
+                         0 : inl ([], ELet "X"%string (ELit 0%Z) (EVar 0), [], [], false) ||||
+                         1 : inl ([], EConcBIF (ELit "send"%string) [EPid 0;ELit 1%Z], [], [], false) ||||
                          nullpool
                       )
                       ([],
-                        0 : ([], ELit 0%Z, []) ||||
-                        1 : ([], EConcBIF (ELit "send"%string) [EPid 0;ELit 1%Z], []) ||||
+                        0 : inl ([], ELit 0%Z, [], [], false) ||||
+                        1 : inl ([], EConcBIF (ELit "send"%string) [EPid 0;ELit 1%Z], [], [], false) ||||
                         nullpool
                       ).
 Proof.
